theory/cwp/geometric.v
@@ -1,6 +1,9 @@
+(** Geometric series definitions and lemmas. *)
+
 Set Implicit Arguments.
 Require Import List.
 Require Import Coq.QArith.QArith.
+Require Import Coq.QArith.Qabs.
 Require Import Coq.micromega.Lqa.
 Require Import Coq.micromega.Lia.
 
@@ -12,6 +15,17 @@ Fixpoint geometric_series (a r : Q) (n : nat) :=
   | O => a
   | S n' => geometric_series a r n' + a * Qpow r n
   end.
+
+(** This is the one being used currently. *)
+Fixpoint geometric_series'' (a r : Q) (n : nat) :=
+  match n with
+  | O => 0
+  | S n' => geometric_series'' a r n' + a * Qpow r n'
+  end.
+
+(** This slightly different series is used instead for wlp. *)
+Definition wlpf_series (a r : Q) (n : nat) :=
+  geometric_series'' a r n + Qpow r n.
 
 Definition geometric_series' (a r : Q) (n : nat) : Q :=
   sum_Q_list (map (fun n => a * Qpow r n) (seq O (S n))).
@@ -27,18 +41,30 @@ Proof.
     set (f := fun n => a * Qpow r n).
     assert (a == f O).
     { unfold f. simpl. field. }
-    rewrite H.
-    rewrite <- Qplus_assoc.
-    rewrite sum_Q_list_l.
-    rewrite Qplus_comm.
-    simpl.
+    rewrite H, <- Qplus_assoc, sum_Q_list_l, Qplus_comm; simpl.
     assert (H0: f O * r * Qpow r n == f (1 + n)%nat).
     { unfold f. simpl. field. }
-    rewrite H0.
-    rewrite <- Qplus_assoc.
-    rewrite sum_Q_list_r.
-    unfold f. simpl. field.
+    rewrite H0, <- Qplus_assoc, sum_Q_list_r.
+    unfold f; simpl; field.
 Qed.
+
+Lemma geometric_series_geometric_series'' (a r : Q) (n : nat) :
+  geometric_series a r n == geometric_series'' a r (S n).
+Proof.
+  induction n; simpl.
+  - lra.
+  - rewrite IHn; reflexivity.
+Qed.
+
+Lemma geometric_series_cons_geometric_series'' (a r : Q) (n : nat) :
+  cons_chain 0 (geometric_series a r) n == geometric_series'' a r n.
+Proof.
+  destruct n.
+  - reflexivity.
+  - apply geometric_series_geometric_series''.
+Qed.
+
+Definition pow_series (a : Q) (i : nat) := Qpow a i.
 
 (* In general we require (|r| < 1) to ensure convergence, but here we
    assume the stronger condition (0 <= r < 1) for simplicity and
@@ -47,6 +73,17 @@ Axiom geometric_series_converges :
   forall a r,
     0 <= r -> r < 1 ->
     converges (geometric_series a r) (a / (1 - r)).
+
+Axiom geometric_series''_converges :
+  forall a r,
+    0 <= r -> r < 1 ->
+    converges (geometric_series'' a r) (a / (1 - r)).
+
+Axiom pow_series_converges :
+  forall a,
+    0 <= a -> a < 1 ->
+    converges (pow_series a) 0.
+
 
 (* Definition converges_from_below (g : nat -> Q) (lim : Q) := *)
 (*   forall eps, 0 < eps -> *)
@@ -68,6 +105,48 @@ Axiom geometric_series_converges :
 (* Definition postfix_series {A : Type} (n : nat) (f : nat -> A) (i : nat) := *)
 (*   f (i-n)%nat. *)
 
+Lemma sum_converges f g limf limg :
+  converges f limf /\ converges g limg ->
+  converges (fun i => f i + g i) (limf + limg).
+Proof.
+  unfold converges.
+  intros [Hf Hg] eps Heps.
+  assert (Heps2: 0 < eps/(2#1)).
+  { apply Qlt_shift_div_l; lra. }
+  specialize (Hf (eps/(2#1)) Heps2).
+  specialize (Hg (eps/(2#1)) Heps2).
+  destruct Hf as [n Hf].
+  destruct Hg as [m Hg].
+  exists (max n m). intros i Hle.
+  assert (Hn: (n <= i)%nat).
+  { eapply Nat.max_lub_l; eauto. }
+  assert (Hm: (m <= i)%nat).
+  { eapply Nat.max_lub_r; eauto. }
+  specialize (Hf i Hn).
+  specialize (Hg i Hm).
+  apply Qle_lt_trans with (Qabs (limf - f i) + Qabs (limg - g i)).
+  - assert (H: limf + limg - (f i + g i) == limf - f i + (limg - g i)).
+    { lra. }
+    rewrite H.
+    apply Qabs_triangle. (* triangle inequality *)
+  - apply Qlt_Qplus_Qdiv2; auto.
+Qed.
+
+Lemma wlpf_series_converges :
+  forall a r,
+    0 <= r -> r < 1 ->
+    converges (wlpf_series a r) (a / (1 - r)).
+Proof.
+  intros a r Hle Hlt.
+  set (f := (geometric_series'' a r)).
+  set (g := fun i => Qpow r i).
+  cut (converges (fun i => f i + g i) (a / (1 - r) + 0)).
+  - intro Hc; eapply Proper_converges; eauto. reflexivity. lra.
+  - apply sum_converges. split.
+    + apply geometric_series''_converges; auto.
+    + apply pow_series_converges; auto.
+Qed.
+
 Lemma geometric_series_succ (a r : Q) (n : nat) :
   a + r * geometric_series a r n == geometric_series a r (S n).
 Proof.
@@ -86,21 +165,17 @@ Proof.
   rewrite sum_Q_list_Qpow; simpl; field.
 Qed.
 
-Lemma geometric_series_supremum (a r : Q) :
-  0 <= a ->
-  0 <= r -> r < 1 ->
-  supremum (a / (1 - r)) (geometric_series a r).
+Lemma geometric_series''_succ (a r : Q) (n : nat) :
+  a + r * geometric_series'' a r n == geometric_series'' a r (S n).
 Proof.
-  intros; apply converges_from_below_supremum.
-  - intro i. simpl.
-    assert (0 <= Qpow r i).
-    { apply Qpow_nonnegative; auto. }
-    assert (0 <= r * Qpow r i). nra. nra.
-  - apply geometric_series_converges; auto.
+  rewrite <- geometric_series_geometric_series''.
+  induction n; simpl.
+  - lra.
+  - rewrite <- IHn; lra.
 Qed.
 
 Lemma geometric_series_monotone (a r : Q) :
-  (0 <= a) -> (0 <= r) ->
+  0 <= a -> 0 <= r ->
   monotone (geometric_series a r).
 Proof.
   intros Hle_a Hle_r n m Hleq. simpl in *.
@@ -115,9 +190,82 @@ Proof.
     assert (0 <= r * Qpow r m); nra.
 Qed.
 
+Lemma geometric_series''_monotone (a r : Q) :
+  0 <= a -> 0 <= r ->
+  monotone (geometric_series'' a r).
+Proof.
+  intros Hle_a Hle_r n m Hleq. simpl in *.
+  induction m. simpl.
+  - inversion Hleq; subst; simpl; lra.
+  - unfold Nat.le in *.
+    destruct (Nat.eqb_spec n (S m)); subst. lra.
+    assert (Hle: (n <= m)%nat). lia.
+    apply IHm in Hle. simpl.
+    generalize (@Qpow_nonnegative r m Hle_r).
+    intro Hle_pow.
+    assert (0 <= r * Qpow r m); nra.
+Qed.
+
+Lemma wlpf_series_succ_le (a r : Q) (i : nat) :
+  0 <= a -> 0 <= r -> r < 1 ->
+  a + r <= 1 ->
+  wlpf_series a r (S i) <= wlpf_series a r i.
+Proof.
+  intros H0 H1 H2 H3.
+  unfold wlpf_series.
+  simpl.
+  cut (a * Qpow r i + r * Qpow r i <= Qpow r i).
+  { lra. }
+  assert (H': a * Qpow r i + r * Qpow r i == (a + r) * Qpow r i).
+  { lra. }
+  rewrite H'; clear H'.
+  apply Qpow_nonnegative with (n:=i) in H1.
+  nra.
+Qed.
+
+Lemma wlpf_series_monotone_decreasing (a r : Q) :
+  0 <= a -> 0 <= r -> r < 1 ->
+  a + r <= 1 ->
+  monotone_decreasing (wlpf_series a r).
+Proof.
+  intros H0 H1 H2 H3 n m Hle.
+  unfold leq in *; simpl in *; unfold Nat.le in Hle.
+  induction m.
+  - destruct n; try lra; lia.
+  - destruct (Nat.eqb_spec n (S m)); subst.
+    + lra.
+    + assert (Hle' : (n <= m)%nat).
+      { lia. }
+      specialize (IHm Hle').
+      eapply Qle_trans; eauto.
+      apply wlpf_series_succ_le; auto.
+Qed.
+
+Lemma geometric_series_supremum (a r : Q) :
+  0 <= a -> 0 <= r -> r < 1 ->
+  supremum (a / (1 - r)) (geometric_series a r).
+Proof.
+  intros; apply converges_from_below_supremum.
+  - intro i. 
+    apply geometric_series_monotone; auto.
+    unfold leq; simpl; unfold Nat.le; lia.
+  - apply geometric_series_converges; auto.
+Qed.
+
+Lemma wlpf_series_infimum (a r : Q) :
+  0 <= a -> 0 <= r -> r < 1 ->
+  a + r <= 1 ->
+  infimum (a / (1 - r)) (wlpf_series a r).
+Proof.
+  intros; apply converges_from_above_infimum.
+  - intro i. simpl.
+    apply wlpf_series_monotone_decreasing; auto.
+    unfold leq; simpl; unfold Nat.le; lia.
+  - apply wlpf_series_converges; auto.
+Qed.
+
 Lemma geometric_supremum (ch : nat -> Q) (a r : Q) :
-  0 <= a ->
-  0 <= r -> r < 1 ->
+  0 <= a -> 0 <= r -> r < 1 ->
   ch ==f geometric_series a r ->
   supremum (a / (1 - r)) ch.
 Proof.
@@ -127,6 +275,33 @@ Proof.
     apply geometric_series_monotone; auto; simpl; unfold Nat.le; lia.
   - eapply Proper_converges; eauto. reflexivity.
     apply geometric_series_converges; auto.
+Qed.
+
+Lemma wlpf_infimum (ch : nat -> Q) (a r : Q) :
+  0 <= a -> 0 <= r -> r < 1 ->
+  a + r <= 1 ->
+  ch ==f wlpf_series a r ->
+  infimum (a / (1 - r)) ch.
+Proof.
+  intros Hle_a Hle_r0 Hle_r1 Hsum Heq.
+  apply converges_from_above_infimum.
+  - intro i. unfold f_Qeq in Heq. rewrite 2!Heq.
+    apply wlpf_series_succ_le; auto.
+  - eapply Proper_converges. intro; apply Heq. reflexivity.
+    apply wlpf_series_converges; auto.
+Qed.
+
+Lemma geometric''_supremum (ch : nat -> Q) (a r : Q) :
+  0 <= a -> 0 <= r -> r < 1 ->
+  ch ==f geometric_series'' a r ->
+  supremum (a / (1 - r)) ch.
+Proof.
+  intros Hle_a Hle_r0 Hle_r1 Heq.
+  apply converges_from_below_supremum.
+  - intro i. unfold f_Qeq in Heq. rewrite 2!Heq.
+    apply geometric_series''_monotone; auto; simpl; unfold Nat.le; lia.
+  - eapply Proper_converges; eauto. reflexivity.
+    apply geometric_series''_converges; auto.
 Qed.
 
 Instance Proper_geometric_series
