theory/cwp/cpGCL.v
@@ -1,7 +1,7 @@
+(** The cpGCL language and associated definitions. *)
+
 Require Import Coq.Program.Basics.
 Require Import Coq.QArith.QArith.
-
-(** The cpGCL language *)
 
 Definition val := bool.
 Definition St : Type := nat -> val.
@@ -48,3 +48,66 @@ Definition expectation {A : Type} (f : A -> Q) := forall x, 0 <= f x.
 
 (** f is a bounded expectation. *)
 Definition bounded_expectation {A : Type} (f : A -> Q) := forall x, 0 <= f x <= 1.
+
+(* Require Import FunctionalExtensionality. *)
+
+(* Lemma kjfg (e e0 : exp) n x : *)
+(*   e (upd n (e0 (upd n (e0 x) x)) (upd n (e0 x) x)) = *)
+(*   e (upd n (e0 x) x). *)
+(* Proof. *)
+(*   f_equal. apply functional_extensionality; intro y. *)
+(*   unfold upd.  *)
+(*   destruct (Nat.eqb_spec y n). *)
+
+(* Lemma upd_twice (n : nat) (e : exp) (x : St) : *)
+(*   (upd n (e (upd n (e x) x)) x) = (upd n (e x) x). *)
+(* Proof. *)
+(*   apply functional_extensionality; intro y. *)
+(*   destruct (e x). unfold upd. *)
+(*   destruct (Nat.eqb_spec y n); subst; auto. *)
+(* Qed. *)
+
+(* Lemma jkdfgdf (f : bool -> bool) : *)
+(*   f = const false \/ f = const true \/ f = id \/ f = negb. *)
+(* Proof. *)
+(*   destruct (f false) eqn:Hf; destruct (f true) eqn:Ht. *)
+(*   - right; left; apply functional_extensionality; intros []; auto. *)
+(*   - right; right; right; apply functional_extensionality; intros []; auto. *)
+(*   - right; right; left; apply functional_extensionality; intros []; auto. *)
+(*   - left; apply functional_extensionality; intros []; auto. *)
+(* Qed. *)
+
+(* Local Open Scope program_scope. *)
+(* Lemma bool_involutive (f : bool -> bool) : *)
+(*   (exists c, f = const c) \/ f ∘ f = id. *)
+(* Proof. *)
+(*   unfold compose, const. *)
+(*   destruct (jkdfgdf f) as [H|[H|[H|H]]]; subst. *)
+(*   - left; exists false; auto. *)
+(*   - left; exists true; auto. *)
+(*   - right; reflexivity. *)
+(*   - right. apply functional_extensionality; intros []; auto. *)
+(* Qed. *)
+
+(* (* Lemma upd_twice (n : nat) (e : exp) (x : St) : *) *)
+(* (*   e (upd n () x) *) *)
+(* (* Proof. *) *)
+(* (*   apply functional_extensionality; intro y. *) *)
+(* (*   destruct (e x). unfold upd. *) *)
+(* (*   destruct (Nat.eqb_spec y n); subst; auto. *) *)
+(* (* Qed. *) *)
+
+(* Lemma upd_shadow n st z y : *)
+(*   upd n y (upd n z st) = upd n y st. *)
+(* Proof. *)
+(*   apply functional_extensionality; intro x. *)
+(*   unfold upd. destruct (Nat.eqb_spec x n); subst; reflexivity. *)
+(* Qed. *)
+
+(* (* Lemma upd_ext (st1 st2 : St) (e : exp) : *) *)
+(* (*   (forall x, st1 x = st2 x) -> *) *)
+(* (*   e st1 = e st2. *) *)
+(* (* Proof. *) *)
+(* (*   apply functional_extensionality in  *) *)
+(* (*   intro Heq.  *) *)
+(* (* Qed. *) *)
