theory/cwp/cwp_cwpf.v
@@ -1,0 +1,684 @@
+(** The relational and functional specifications of CWP coincide when
+    all loops are iid. *)
+
+Set Implicit Arguments.
+
+Require Import Coq.Program.Basics.
+Require Import List.
+Require Import Nat.
+Require Import Coq.QArith.QArith.
+Require Import Coq.micromega.Lqa.
+Require Import Coq.micromega.Lia.
+Local Open Scope program_scope.
+Import ListNotations.
+
+Require Import cpGCL.
+Require Import cwp.
+Require Import cwpf_infer.
+Require Import geometric.
+Require Import order.
+Require Import Q.
+
+Open Scope cpGCL_scope.
+Open Scope Q_scope.
+
+Lemma wpf_linear c f g st :
+  wpf c (fun st => f st + g st) st == wpf c f st + wpf c g st.
+Proof.
+  revert f g st.
+  induction c; intros f g st; simpl.
+  - reflexivity.
+  - unfold const; lra.
+  - reflexivity.
+  - unfold compose. rewrite <- IHc1.
+    apply Proper_wpf; auto.
+    intros ?; apply IHc2.
+  - destruct (e st); auto.
+  - rewrite IHc1, IHc2. lra.
+  - destruct (Qeq_dec (wpf c (fun st => if e st then 1 else 0) st) 1).
+    + rewrite q, Qminus_cancel, 3!Qdiv_0_den; lra.
+    + assert (H0: forall a b c, ~ c == 0 -> a / c + b / c == (a + b) / c).
+      { intros. field; auto. }
+      rewrite H0.
+      * rewrite <- IHc. apply Qeq_Qdiv.
+        ++ apply Proper_wpf; auto.
+           intro x; destruct (e x); lra.
+        ++ reflexivity.
+      * lra.
+  - destruct (e st); lra.
+Qed.
+
+Lemma wpf_linear' c (e : exp) f g st :
+  wpf c (fun x => if e x then f x else g x) st ==
+  wpf c (fun x => if e x then f x else 0) st +
+  wpf c (fun x => if e x then 0 else g x) st.
+Proof.
+  rewrite <- wpf_linear; apply Proper_wpf; auto.
+  intro x; destruct (e x); lra.
+Qed.
+
+Lemma wpf_strict c f x :
+  f ==f const 0 ->
+  wpf c f x == 0.
+Proof.
+  revert f x.
+  induction c; simpl; unfold const in *; intros f x Heq; auto; try reflexivity.
+  - unfold compose; auto.
+  - destruct (e x); auto.
+  - rewrite IHc1, IHc2; auto; lra.
+  - rewrite IHc.
+    + apply Qdiv_0_num.
+    + intro y; destruct (e y); auto; reflexivity.
+  - destruct (e x); auto; reflexivity.
+Qed.
+
+Lemma wpf_bounded c f :
+  wf_cpGCL c ->
+  (forall x, f x <= 1) ->
+  forall x, wpf c f x <= 1.
+Proof.
+  revert f.
+  induction c; intros f Hwf Hle x; simpl; inversion Hwf; subst; auto.
+  - unfold const; lra.
+  - apply IHc1; auto.
+  - destruct (e x).
+    + apply IHc1; auto.
+    + apply IHc2; auto.
+  - specialize (IHc1 f H3 Hle x); specialize (IHc2 f H4 Hle x); nra.
+  - set (ea := wpf c (fun st => if e st then 0 else f st) x).
+    set (eb := wpf c (fun st => if e st then 1 else 0) x).
+    assert (eb <= 1).
+    { apply IHc; auto.
+      intro y; destruct (e y); lra. }
+    destruct (Qeq_dec eb 1).
+    { rewrite q, Qminus_cancel, Qdiv_0_den; lra. }
+    apply ratio_Qle_sum. lra.
+    rewrite Qmult_1_r.
+    assert (ea <= 1).
+    { apply IHc; auto.
+      intro y; destruct (e y); auto; lra. }
+    assert (H': eb == wpf c (fun x => if e x then const 1 x else 0) x).
+    { apply Proper_wpf; auto. intro y; destruct (e y); reflexivity. }
+    rewrite H'; clear H'.
+    unfold ea.
+    rewrite Qplus_comm.
+    rewrite <- wpf_linear'.
+    apply IHc; auto.
+    intro y; destruct (e y); auto.
+    unfold const; lra.
+  - destruct (e x); auto; lra.
+Qed.
+
+Lemma wlpf_linear c f g st :
+  wlpf c (fun st => f st + g st) st == wpf c f st + wlpf c g st.
+Proof.
+  revert f g st.
+  induction c; intros f g st; simpl.
+  - reflexivity.
+  - unfold const; lra.
+  - reflexivity.
+  - unfold compose. rewrite <- IHc1.
+    apply Proper_wlpf; auto.
+    intros ?; apply IHc2.
+  - destruct (e st); auto.
+  - rewrite IHc1, IHc2. lra.
+  - destruct (Qeq_dec (wpf c (fun st => if e st then 1 else 0) st) 1).
+    + rewrite Qeq_eq_bool; auto.
+      rewrite q, Qminus_cancel, Qdiv_0_den; lra.
+    + rewrite Qeq_bool_false; auto.
+      assert (H0: forall a b c, ~ c == 0 -> a / c + b / c == (a + b) / c).
+      { intros. field; auto. }
+      rewrite H0.
+      * rewrite <- IHc. apply Qeq_Qdiv.
+        ++ apply Proper_wlpf; auto.
+           intro x; destruct (e x); lra.
+        ++ reflexivity.
+      * lra.
+  - destruct (e st); lra.
+Qed.
+
+Lemma wlpf_linear' c (e : exp) f g st :
+  wlpf c (fun st' => if e st' then f st' else g st') st ==
+  wpf c (fun st' => if e st' then f st' else 0) st +
+  wlpf c (fun st' => if e st' then 0 else g st') st.
+Proof.
+  rewrite <- wlpf_linear; apply Proper_wlpf; auto.
+  intro x; destruct (e x); lra.
+Qed.
+
+Lemma wlpf_bounded c f :
+  wf_cpGCL c ->
+  (forall x, f x <= 1) ->
+  forall x, wlpf c f x <= 1.
+Proof.
+  revert f.
+  induction c; intros f Hwf Hle x; simpl; inversion Hwf; subst; auto.
+  - unfold const; lra.
+  - apply IHc1; auto.
+  - destruct (e x).
+    + apply IHc1; auto.
+    + apply IHc2; auto.
+  - specialize (IHc1 f H3 Hle x); specialize (IHc2 f H4 Hle x); nra.
+  - set (ea := wlpf c (fun st => if e st then 0 else f st) x).
+    set (eb := wpf c (fun st => if e st then 1 else 0) x).
+    assert (eb <= 1).
+    { apply wpf_bounded; auto.
+      intro y; destruct (e y); lra. }
+    destruct (Qeq_dec eb 1).
+    { rewrite q. simpl. lra. }
+    rewrite Qeq_bool_false; auto.
+    apply ratio_Qle_sum. lra.
+    rewrite Qmult_1_r.
+    assert (ea <= 1).
+    { apply IHc; auto.
+      intro y; destruct (e y); auto; lra. }
+    assert (H': eb == wpf c (fun x => if e x then const 1 x else 0) x).
+    { apply Proper_wpf; auto. intro y; destruct (e y); reflexivity. }
+    rewrite H'; clear H'.
+    unfold ea.
+    rewrite Qplus_comm.
+    rewrite <- wlpf_linear'.
+    apply IHc; auto.
+    intro y; destruct (e y); auto.
+    unfold const; lra.
+  - destruct (e x); auto; lra.
+Qed.
+
+Lemma wpf_expectation c f :
+  wf_cpGCL c ->
+  expectation f ->
+  expectation (wpf c f).
+Proof.
+  revert f.
+  induction c; intros f Hwf Hexp; simpl; inversion Hwf; subst; auto.
+  - unfold const; intros ?; lra.
+  - intros ?; apply Hexp.
+  - apply IHc1; auto.
+  - intro x; destruct (e x).
+    + apply IHc1; auto.
+    + apply IHc2; auto.
+  - intro x.
+    specialize (IHc1 f H3 Hexp x); specialize (IHc2 f H4 Hexp x).
+    nra.
+  - intro x. simpl.
+    assert (wpf c (fun st => if e st then 1 else 0) x <= 1).
+    { apply wpf_bounded; auto.
+      intro st; destruct (e st); auto; lra. }
+    destruct (Qeq_dec (wpf c (fun st => if e st then 1 else 0) x) 1).
+    + rewrite q, Qminus_cancel, Qdiv_0_den; lra.
+    + apply Qle_shift_div_l. lra. rewrite Qmult_0_l. apply IHc; auto.
+      intro st; destruct (e st); auto; lra.
+  - intro x; destruct (e x); auto; lra.
+Qed.
+
+Lemma wlpf_expectation c f :
+  wf_cpGCL c ->
+  expectation f ->
+  expectation (wlpf c f).
+Proof.
+  revert f.
+  induction c; intros f Hwf Hexp; simpl; inversion Hwf; subst; auto.
+  - unfold const; intros ?; lra.
+  - intros ?; apply Hexp.
+  - apply IHc1; auto.
+  - intro x; destruct (e x).
+    + apply IHc1; auto.
+    + apply IHc2; auto.
+  - intro x.
+    specialize (IHc1 f H3 Hexp x); specialize (IHc2 f H4 Hexp x).
+    nra.
+  - intro x. simpl.
+    assert (wpf c (fun st => if e st then 1 else 0) x <= 1).
+    { apply wpf_bounded; auto.
+      intro st; destruct (e st); auto; lra. }
+    destruct (Qeq_dec (wpf c (fun st => if e st then 1 else 0) x) 1).
+    + apply Qeq_bool_iff in q. rewrite q; lra.
+    + rewrite Qeq_bool_false; auto; apply Qle_shift_div_l.
+      lra. rewrite Qmult_0_l. apply IHc; auto.
+      intro st; destruct (e st); auto; lra.
+  - intro x; destruct (e x); auto; lra.
+Qed.
+
+Lemma wlpf_bounded_expectation c f :
+  wf_cpGCL c ->
+  bounded_expectation f ->
+  bounded_expectation (wlpf c f).
+Proof.
+  revert f.
+  induction c; intros f Hwf Hexp; simpl; inversion Hwf; subst; auto.
+  - unfold const; intros ?; lra.
+  - intros ?; apply Hexp.
+  - apply IHc1; auto.
+  - intro x; destruct (e x).
+    + apply IHc1; auto.
+    + apply IHc2; auto.
+  - intro x.
+    specialize (IHc1 f H3 Hexp x); specialize (IHc2 f H4 Hexp x).
+    nra.
+  - intro x. simpl.
+    assert (wpf c (fun st => if e st then 1 else 0) x <= 1).
+    { apply wpf_bounded; auto.
+      intro st; destruct (e st); auto; lra. }
+    destruct (Qeq_dec (wpf c (fun st => if e st then 1 else 0) x) 1).
+    + apply Qeq_bool_iff in q. rewrite q; lra.
+    + rewrite Qeq_bool_false; auto; split.
+      * apply Qle_shift_div_l. lra.
+        rewrite Qmult_0_l; apply IHc; auto.
+        intro st; destruct (e st); auto; lra.
+      * admit.
+  - intro x; destruct (e x); auto; lra.
+Admitted.
+
+Lemma wpf_chain_geometric_series f e c st i :
+  iid_wpf e c ->
+  wpf (unroll e c i) f st ==
+  geometric_series'' (wpf c (fun x => if e x then 0 else f x) st)
+                     (wpf c (indicator e) st) i.
+Proof.
+  intro Hiid; induction i.
+  - reflexivity.
+  - rewrite Hiid.
+    rewrite IHi.
+    rewrite Qplus_comm.
+    apply geometric_series''_succ.
+Qed.
+
+Lemma wlpf_chain_series f e c st i :
+  iid_wlpf e c ->
+  wlpf (unroll e c i) f st ==
+  wlpf_series (wlpf c (fun x => if e x then 0 else f x) st)
+              (wpf c (indicator e) st) i.
+  (* geometric_series'' (wlpf c (fun x => if e x then 0 else f x) st) *)
+  (*                    (wpf c (indicator e) st) i + *)
+  (* Qpow (wpf c (indicator e) st) i. *)
+Proof.
+  unfold wlpf_series; intro Hiid; induction i.
+  - reflexivity.
+  - rewrite Hiid, IHi, Qplus_comm.
+    simpl.
+    (* set (a := wlpf c (fun x : St => if e x then 0 else f x) st). *)
+    (* set (r := wpf c (indicator e) st). *)
+    rewrite Qmult_plus_distr_r, Qplus_assoc, geometric_series''_succ.
+    reflexivity.
+Qed.
+
+Lemma wf_unroll c e i :
+  wf_cpGCL c ->
+  wf_cpGCL (unroll e c i).
+Proof. induction i; repeat constructor; auto. Qed.
+
+(* Lemma kdfgfsdf c e st : *)
+(*   wf_cpGCL c -> *)
+(*   wpf c (indicator e) st + wpf c (neg_indicator e) st == 1. *)
+(* Admitted. *)
+
+Lemma wpf_monotone c :
+  wf_cpGCL c ->
+  monotone (wpf c).
+Proof.
+  induction c; unfold monotone, leq; simpl;
+    intros Hwf f g Hleq x; auto; inversion Hwf; subst.
+  - lra.
+  - apply IHc1; auto; apply IHc2; auto.
+  - destruct (e x).
+    + apply IHc1; auto.
+    + apply IHc2; auto.
+  - specialize (IHc1 H3 f g Hleq x).
+    specialize (IHc2 H4 f g Hleq x).
+    unfold leq in *; simpl in *; nra.
+  - specialize (IHc H0).
+    cut (wpf c (fun st' : St => if e st' then 0 else f st') x <=
+         wpf c (fun st' : St => if e st' then 0 else g st') x).
+    { intros.
+      destruct (Qeq_dec (wpf c (fun x => if e x then 1 else 0) x) 1).
+      { rewrite q, Qminus_cancel, 2!Qdiv_0_den; lra. }
+      assert (wpf c (fun x => if e x then 1 else 0) x <= 1).
+      { apply wpf_bounded; auto.
+        intro y; destruct (e y); lra. }
+      apply Qle_Qdiv; auto.
+      lra. }
+    apply IHc; simpl.
+    intro y; destruct (e y); auto; lra.
+  - destruct (e x); auto; lra.
+Qed.
+
+(* Lemma wpf_decreasing c f x : *)
+(*   wpf c f x <= f x. *)
+(* Proof. *)
+(*   (* revert f x. *) *)
+(*   (* induction c; intros f x Hexp; simpl. *) *)
+(*   (* - lra. *) *)
+(*   (* - apply Hexp. *) *)
+(*   (* -  *) *)
+(* Admitted. *)
+
+(* Lemma kdfgf c e st : *)
+(*   wf_cpGCL c -> *)
+(*   (forall f, f ==f indicator e -> wpf c f st == 1) -> *)
+(*   (* forall g, g ==f neg_indicator e -> wpf c g st == 0. *) *)
+(*   forall f g, expectation g -> (forall x, g x <= if e x then 0 else f x) -> *)
+(*          wpf c g st == 0. *)
+(* Proof. *)
+(*   revert e st. *)
+(*   induction c; intros G st Hwf Heq f g Hexp Hle. *)
+(*   - simpl in *. *)
+(*     specialize (Heq (indicator G) (f_Qeq_refl _)). *)
+(*     unfold indicator in *. *)
+(*     (* rewrite Heq'. *) *)
+(*     specialize (Hle st). *)
+(*     destruct (G st). *)
+(*     + specialize (Hexp st); lra. *)
+(*     + lra. *)
+(*   - reflexivity. *)
+(*   - simpl in *. admit. *)
+(*   - simpl in *. *)
+(*     unfold compose in *. *)
+(*     inversion Hwf; subst. *)
+(*     apply IHc1 with (e:=G) (f:=f); auto. *)
+(*     + intros h Hh. *)
+(*       specialize (Heq h Hh). *)
+(*       assert (Hle': 1 <= wpf c1 h st). *)
+(*       { apply Qle_trans with (wpf c1 (wpf c2 h) st). *)
+(*         - lra. *)
+(*         - apply wpf_monotone; auto. *)
+(*           intro s; simpl. *)
+(*           apply wpf_decreasing. } *)
+(*       assert (wpf c1 h st <= 1). *)
+(*       { apply wpf_bounded; auto. *)
+(*         intro y. rewrite Hh. unfold indicator. destruct (G y); lra. } *)
+(*       lra. *)
+(*     + apply wpf_expectation; auto. *)
+(*     + intro x; specialize (Hle x). *)
+(*       apply Qle_trans with (g x); auto. *)
+(*       apply wpf_decreasing. *)
+(*   - admit. (* TODO *) *)
+(*   - admit. *)
+(*   - admit. *)
+(*   - simpl in *. *)
+(*     specialize (Heq (indicator G) (f_Qeq_refl _)). *)
+(*     unfold indicator in Heq. *)
+(*     destruct (e st); try lra. *)
+(*     specialize (Hle st). destruct (G st). *)
+(*     + specialize (Hexp st); lra. *)
+(*     + lra. *)
+(* Admitted. *)
+
+Lemma asdkdf c (e : exp) st :
+  wf_cpGCL c ->
+  wpf c (fun x => if e x then 1 else 0) st == 1 ->
+  wpf c (fun x => if e x then 0 else 1) st == 0.
+Proof.
+  unfold indicator.
+  set (a := wpf c (fun st : St => if e st then 1 else 0) st).
+  set (b := wpf c (fun st : St => if e st then 0 else 1) st).
+  intros Hwf Heq.
+  cut (a + b <= 1).
+  { intros.
+    assert (0 <= a).
+    { apply wpf_expectation; auto.
+      intro y; destruct (e y); lra. }
+    assert (0 <= b).
+    { apply wpf_expectation; auto.
+      intro y; destruct (e y); auto; lra. }
+    lra. }
+  assert (a == wpf c (fun x => if e x then const 1 x else 0) st).
+  { apply Proper_wpf; auto. intro y; destruct (e y); reflexivity. }
+  rewrite H. unfold b.
+  rewrite <- wpf_linear'.
+  apply wpf_bounded; auto.
+  intro y; destruct (e y); auto; unfold const; lra.
+Qed.
+
+(* Lemma sdfasdfsdkdf c (e : exp) f st : *)
+(*   wpf c (fun x => if e x then 1 else 0) st == 0 -> *)
+(*   wpf c (fun x => if e x then f x else 0) st == 0. *)
+(* Proof. *)
+
+
+(* Lemma djkifg c f g st : *)
+(*   wpf c f st == 0 -> *)
+(*   wpf c (fun x => f st * g st) st == 0. *)
+(* Proof. *)
+(*   revert f g st. *)
+(*   induction c; simpl; intros f g st Heq; auto. *)
+(*   - rewrite Heq; lra. *)
+(*   -  *)
+
+
+(* Lemma djkifg c (e : exp) f st : *)
+(*   wpf c (fun x => if e x then 0 else f x) st == *)
+(*   wpf c (fun x => if e x then 0 else 1) st * wpf c f st. *)
+(* Proof. *)
+  
+
+Lemma sdfasdkdf c (e : exp) f st :
+  wpf c (fun x => if e x then 0 else 1) st == 0 ->
+  wpf c (fun x => if e x then 0 else f x) st == 0.
+Proof.
+Admitted.
+
+(* Lemma asdkdfgf c e st f : *)
+(*   wf_cpGCL c -> *)
+(*   expectation f -> *)
+(*   wpf c (indicator e) st == 1 -> *)
+(*   wpf c (fun x => if e x then 0 else f x) st == 0. *)
+(* Proof. *)
+(*   unfold indicator. *)
+(*   set (a := wpf c (fun st : St => if e st then 1 else 0) st). *)
+(*   set (b := wpf c (fun st : St => if e st then 0 else f st) st). *)
+(*   intros Hwf Hexp Heq. *)
+(*   cut (a + b <= 1). *)
+(*   { intros. *)
+(*     assert (0 <= a). *)
+(*     { apply wpf_expectation; auto. *)
+(*       intro y; destruct (e y); lra. } *)
+(*     assert (0 <= b). *)
+(*     { apply wpf_expectation; auto. *)
+(*       intro y; destruct (e y); auto; lra. } *)
+(*     lra. } *)
+(*   (* wpf_linear' *) *)
+(*   assert (a == wpf c (fun x => if e x then const 1 x else 0) st). *)
+(*   { apply Proper_wpf; auto. intro y; destruct (e y); reflexivity. } *)
+(*   rewrite H. unfold b. *)
+(*   rewrite <- wpf_linear'. *)
+(*   apply wpf_bounded; auto. *)
+(*   intro y; destruct (e y); auto. *)
+  
+(*   revert e st f. *)
+(*   induction c; simpl; unfold indicator; *)
+(*     intros G st f Hwf Heq; inversion Hwf; subst. *)
+(*   - intro H; destruct (G st); lra. *)
+(*   - intro H; inversion H. *)
+(*   - intro H; destruct (G (upd n (e st) st)); lra. *)
+(*   - unfold compose. intro H. *)
+
+(*   (* revert e st f. *) *)
+(*   (* induction c; simpl; unfold indicator; intros G st f Hwf Heq. *) *)
+(*   (* assert (H0: forall x, indicator G x == (if G x then 1 else 0)). *) *)
+(*   (* { intros; reflexivity. } *) *)
+(*   (* - (* specialize (Heq (indicator G) H0). *) *) *)
+(*   (*   (* unfold indicator in Heq. *) *) *)
+(*   (*   destruct (G st); lra. *) *)
+(*   (* - reflexivity. *) *)
+(*   (* - destruct (G (upd n (e st) st)); lra. *) *)
+(*   (* - unfold compose in *. *) *)
+(*   (*   inversion Hwf; subst. *) *)
+(*   (*   apply kdfgf with (e:=G); auto. *) *)
+(*   (*   intros. *) *)
+(*   (*   rewrite <- Heq. *) *)
+(*   (*   apply Proper_wpf; auto. *) *)
+(*   (*   intro. rewrite H. unfold indicator. *) *)
+(*   (*   apply Heq. *) *)
+(*   intros Hwf Hexp Heq. *)
+(*   apply kdfgf with (e:=e) (f:=f); auto. *)
+(*   - intros g Heq'. *)
+(*     rewrite <- Heq. *)
+(*     eapply Proper_wpf; auto. *)
+(*   - intro x.  *)
+(*     destruct (e x); auto; lra. *)
+(*   - intro; lra. *)
+(* Qed. *)
+
+Lemma asdkdfgf' c e st f :
+  wf_cpGCL c ->
+  (wpf c (indicator e) st == 1) ->
+  wlpf c (fun x => if e x then 0 else f x) st == 0.
+Proof.
+Admitted.
+
+Lemma wpf_unroll_const_0 c e x i f :
+  wf_cpGCL c ->
+  iid_wpf e c ->
+  expectation f ->
+  wpf c (indicator e) x == 1 ->
+  wpf (unroll e c i) f x == (const 0) i.
+Proof.
+  revert c e x f; unfold indicator.
+  induction i; intros c e x f Hwf Hiid Hexp Heq; unfold compose, const.
+  - reflexivity.
+  - rewrite Hiid.
+    rewrite IHi; auto.
+    unfold const. rewrite Qmult_0_r, Qplus_0_l.
+    apply sdfasdkdf; auto.
+    apply asdkdf; auto.
+Qed.
+
+Lemma wlpf_unroll_const_1 c e x i f :
+  wf_cpGCL c ->
+  iid_wlpf e c ->
+  wpf c (indicator e) x == 1 ->
+  wlpf (unroll e c i) f x == (const 1) i.
+Proof.
+  revert c e x f; unfold indicator.
+  induction i; intros c e x f Hwf Hiid Heq; unfold compose, const.
+  - reflexivity.
+  - rewrite Hiid. rewrite IHi; auto.
+    unfold const. rewrite Qmult_1_r.
+    rewrite Heq. rewrite asdkdfgf'; auto; lra.
+Qed.
+
+(** wp and wpf coincide when every loop in the program is iid. *)
+Lemma wp_wpf (c : cpGCL) (f : St -> Q) :
+  wf_cpGCL c ->
+  iid_cpGCL c ->
+  expectation f ->
+  wp c f (wpf c f).
+Proof.
+  revert f.
+  induction c; intros f Hwf Hiid Hexp; simpl;
+    inversion Hwf; inversion Hiid; subst;
+      try solve [econstructor; auto; reflexivity].
+  - unfold compose.
+    econstructor; auto.
+    apply IHc1; auto.
+    apply wpf_expectation; auto.
+    reflexivity.
+  - set (ch := flip wpf f ∘ unroll e c).
+    apply wp_while with (ch := ch).
+    + reflexivity.
+    + intro n.
+      eexists. split.
+      * apply IHc; auto.
+        unfold ch.
+        unfold compose, flip.
+        apply wpf_expectation; auto.
+        apply wf_unroll; auto.
+      * intro x. unfold ch. unfold compose. unfold flip.
+        simpl. reflexivity.
+    + apply supremum_pointwise; intro x.
+      assert (Hle: wpf c (indicator e) x <= 1).
+      { apply wpf_bounded; auto.
+        intro y; unfold indicator; destruct (e y); lra. }
+      destruct (Qeq_dec (wpf c (indicator e) x) 1).
+      -- unfold indicator in *.
+         eapply Proper_supremum_Q.
+         rewrite q, Qminus_cancel, Qdiv_0_den; reflexivity.
+         intro i. unfold app_chain, flip.
+         unfold ch. unfold compose, flip.
+         destruct H5; apply wpf_unroll_const_0; auto.
+         apply const_supremum.
+         intro i; unfold const. apply Qeq_equ; reflexivity.
+      -- apply geometric''_supremum.
+           ++ apply wpf_expectation; auto.
+              intro y; destruct (e y); auto; lra.
+           ++ apply wpf_expectation; auto.
+              intro y; destruct (e y); auto; lra.
+           ++ unfold indicator in *; lra.
+           ++ intro i; destruct H5; apply wpf_chain_geometric_series; auto.
+Qed.
+
+(** wlp and wlpf coincide when every loop in the program is iid. *)
+Lemma wlp_wlpf (c : cpGCL) (f : St -> Q) :
+  wf_cpGCL c ->
+  iid_cpGCL c ->
+  bounded_expectation f ->
+  wlp c f (wlpf c f).
+Proof.
+  revert f.
+  induction c; intros f Hwf Hiid Hexp; simpl;
+    inversion Hwf; inversion Hiid; subst; try solve [constructor; reflexivity].
+  - unfold compose.
+    econstructor; auto.
+    apply IHc1; auto.
+    apply wlpf_bounded_expectation; auto.
+    reflexivity.
+  - econstructor; eauto; reflexivity.
+  - econstructor; eauto. reflexivity.
+  - set (ch := flip wlpf f ∘ unroll e c).
+    apply wlp_while with (ch := ch).
+    + reflexivity.
+    + intro n.
+      eexists. split.
+      * apply IHc; auto.
+        unfold ch.
+        unfold compose, flip.
+        apply wlpf_bounded_expectation; auto.
+        apply wf_unroll; auto.
+      * intro x. unfold ch. unfold compose. unfold flip.
+        simpl. reflexivity.
+    + apply infimum_pointwise; intro x.
+      assert (Hle: wpf c (indicator e) x <= 1).
+      { apply wpf_bounded; auto.
+        intro y; unfold indicator; destruct (e y); lra. }
+      destruct (Qeq_dec (wpf c (indicator e) x) 1).
+      -- unfold indicator in *.
+         eapply Proper_infimum_Q.
+         rewrite Qeq_eq_bool. reflexivity. auto.
+         intro i. unfold app_chain, ch, flip, compose.
+         destruct H5; apply wlpf_unroll_const_1; auto.
+         apply const_infimum.
+         intro; apply Qeq_equ; reflexivity.
+      -- eapply Proper_infimum_Q. rewrite Qeq_bool_false; auto.
+         reflexivity. reflexivity.
+         apply wlpf_infimum.
+         ++ apply wlpf_expectation; auto.
+            intro y; destruct (Hexp y); destruct (e y); auto; lra.
+         ++ apply wpf_expectation; auto.
+            intro y; destruct (Hexp y); destruct (e y); auto; lra.
+         ++ unfold indicator in *; lra.
+         ++ set (a := wlpf c (fun st' : St => if e st' then 0 else f st') x).
+            set (b := wpf c (fun st' : St => if e st' then 1 else 0) x).
+            assert (H: b == wpf c (fun y => if e y then const 1 y else 0) x).
+            { eapply Proper_wpf; auto. intro y; destruct (e y); reflexivity. }
+            rewrite H; clear H.
+            rewrite Qplus_comm; unfold a.
+            rewrite <- wlpf_linear'.
+            apply wlpf_bounded; auto.
+            intro y; destruct (Hexp y); destruct (e y); auto; unfold const; lra.
+         ++ intro i; destruct H5; apply wlpf_chain_series; auto.
+Qed.
+
+Theorem cwp_cwpf (c : cpGCL) (f : St -> Q) :
+  wf_cpGCL c ->
+  iid_cpGCL c ->
+  expectation f ->
+  cwp c f (cwpf c f).
+Proof.
+  intros Hwf Hiid Hexp; unfold cwp.
+  exists (wpf c f). exists (wlpf c (const 1)); split.
+  - split.
+    + apply wp_wpf; auto.
+    + apply wlp_wlpf; auto.
+      intro; unfold const; lra.
+  - reflexivity.
+Qed.
