theory/cwp/cwpf_infer.v
@@ -1,0 +1,175 @@
+(** Compilation+inference agrees with functional CWP (always). *)
+
+Set Implicit Arguments.
+Require Import Coq.Program.Basics.
+Require Import Coq.QArith.QArith.
+Require Import Coq.micromega.Lqa.
+Require Import Coq.micromega.Lia.
+Require Import ExtLib.Data.Monads.StateMonad.
+Local Open Scope program_scope.
+
+Require Import compile.
+Require Import cpGCL.
+Require Import cwp.
+Require Import infer.
+Require Import order.
+Require Import Q.
+Require Import tree.
+
+Lemma wpf_infer_f c f n :
+  wf_cpGCL c ->
+  wpf c f ==f infer_f f ∘ evalCompile c n.
+Proof.
+  revert n f.
+  induction c; intros m f Hwf st;
+    unfold evalCompile, evalState, compose; simpl; inversion Hwf; subst.
+  - reflexivity.
+  - rewrite Qdiv_0_num; reflexivity.
+  - reflexivity.
+  - unfold compose.
+    unfold compose, f_Qeq, evalCompile, evalState in *.
+    destruct (runState (compile c1) m) eqn:Hc1.
+    destruct (runState (compile c2) n) eqn:Hc2.
+    specialize (IHc1 m (wpf c2 f) H1 st).
+    rewrite IHc1. simpl.
+    rewrite Hc1. simpl.
+    unfold kcomp. simpl.
+    rewrite <- infer_f_bind. unfold compose. simpl.
+    + apply infer_f_proper; intro x.
+      specialize (IHc2 n f H2 x).
+      rewrite IHc2, Hc2; reflexivity.
+    + intros l x Hbound. apply not_in_not_bound_and_not_free. split.
+      * apply free_in_not_free_in; intro HC.
+        eapply compile_free_in_0 in Hc2; eauto. subst.
+        eapply compile_bound_labels in Hc1; eauto; lia.
+      * apply bound_in_not_bound_in; intro HC.
+        eapply compile_bound_labels in Hc2; eauto.
+        eapply compile_bound_labels in Hc1; eauto.
+        lia.
+  - unfold compose, evalCompile, evalState, f_Qeq in *.
+    destruct (runState (compile c1) m) eqn:Hc1.
+    destruct (runState (compile c2) n) eqn:Hc2.
+    simpl; destruct (e st).
+    + rewrite IHc1, Hc1; auto; reflexivity.
+    + rewrite IHc2, Hc2; auto; reflexivity.
+  - unfold compose, evalCompile, evalState, f_Qeq in *.
+    destruct (runState (compile c1) m) eqn:Hc1.
+    destruct (runState (compile c2) n) eqn:Hc2.
+    rewrite IHc1, Hc1, IHc2, Hc2; auto; reflexivity.
+  - destruct (runState (compile c) (S m)) eqn:Hc.
+    pose proof IHc as IHc'.
+    specialize (IHc (S m) f H0 st).
+    unfold compose, evalCompile, evalState, f_Qeq in *.
+    rewrite Hc in IHc. simpl in *.
+    set (g := fun st' => if e st' then 0 else f st').
+    set (h := fun st' => if e st' then 1 else 0).
+    set (k := fun st' => if e st' then Fail St (S m) else Leaf st').
+    cut (wpf c g st == infer_f f (tree_bind (t st) k)).
+    cut (wpf c h st == infer_fail (S m) (tree_bind (t st) k)).
+    { intros H1 H2; rewrite H1, H2; reflexivity. }
+    + unfold h. unfold k.
+      rewrite infer_fail_tree_bind_infer_f.
+      specialize (IHc' (S m) (fun st => if e st then 1 else 0) H0 st).
+      rewrite Hc in IHc'. simpl in IHc'.
+      apply IHc'.
+      apply label_in_not_in; intro HC. apply label_in_bound_or_free in HC.
+      destruct HC as [HC|HC].
+      * eapply compile_bound_labels in Hc; eauto; lia.
+      * eapply compile_free_in_0 in Hc; eauto; lia.
+      * eapply compile_wf_tree'; eauto.
+    + specialize (IHc' (S m) g H0 st).
+      rewrite IHc'. rewrite Hc. simpl.
+      unfold g. unfold k.
+      rewrite infer_f_bind_fail.
+      * reflexivity.
+      * apply bound_in_not_bound_in; intro HC.
+        eapply compile_bound_labels in Hc; eauto; lia.
+  - destruct (e st); reflexivity.
+Qed.
+
+Lemma wlpf_infer_f_lib c f n :
+  wf_cpGCL c ->
+  wlpf c f ==f infer_f_lib f ∘ evalCompile c n.
+Proof.
+  revert n f.
+  induction c; intros m f Hwf st;
+    unfold evalCompile, evalState, compose; simpl; inversion Hwf; subst.
+  - reflexivity.
+  - rewrite Nat.eqb_refl; reflexivity.
+  - reflexivity.
+  - unfold compose.
+    unfold compose, f_Qeq, evalCompile, evalState in *.
+    destruct (runState (compile c1) m) eqn:Hc1.
+    destruct (runState (compile c2) n) eqn:Hc2.
+    specialize (IHc1 m (wlpf c2 f) H1 st).
+    rewrite IHc1. simpl.
+    rewrite Hc1. simpl.
+    unfold kcomp. simpl.
+    rewrite <- infer_f_lib_bind. unfold compose. simpl.
+    + apply infer_f_lib_proper; intro x.
+      specialize (IHc2 n f H2 x).
+      rewrite IHc2, Hc2; reflexivity.
+    + intros l x Hbound. apply not_in_not_bound_and_not_free. split.
+      * apply free_in_not_free_in; intro HC.
+        eapply compile_free_in_0 in Hc2; eauto. subst.
+        eapply compile_bound_labels in Hc1; eauto; lia.
+      * apply bound_in_not_bound_in; intro HC.
+        eapply compile_bound_labels in Hc2; eauto.
+        eapply compile_bound_labels in Hc1; eauto.
+        lia.
+  - unfold compose, evalCompile, evalState, f_Qeq in *.
+    destruct (runState (compile c1) m) eqn:Hc1.
+    destruct (runState (compile c2) n) eqn:Hc2.
+    simpl; destruct (e st).
+    + rewrite IHc1, Hc1; auto; reflexivity.
+    + rewrite IHc2, Hc2; auto; reflexivity.
+  - unfold compose, evalCompile, evalState, f_Qeq in *.
+    destruct (runState (compile c1) m) eqn:Hc1.
+    destruct (runState (compile c2) n) eqn:Hc2.
+    rewrite IHc1, Hc1, IHc2, Hc2; auto; reflexivity.
+  - destruct (runState (compile c) (S m)) eqn:Hc.
+    pose proof IHc as IHc'.
+    specialize (IHc (S m) f H0 st).
+    unfold compose, evalCompile, evalState, f_Qeq in *.
+    rewrite Hc in IHc. simpl in *.
+    set (g := fun st' => if e st' then 0 else f st').
+    set (h := fun st' => if e st' then 1 else 0).
+    set (k := fun st' => if e st' then Fail St (S m) else Leaf st').
+    cut (wlpf c g st == infer_f_lib f (tree_bind (t st) k)).
+    cut (wpf c h st == infer_fail (S m) (tree_bind (t st) k)).
+    { intros H1 H2. rewrite H1.
+    destruct (Qeq_dec (infer_fail (S m) (tree_bind (t st) k)) 1).
+    { rewrite Qeq_eq_bool; auto; reflexivity. }
+    rewrite Qeq_bool_false; auto.
+    rewrite H1, H2. reflexivity. }
+    + unfold h. unfold k.
+      rewrite infer_fail_tree_bind_infer_f.
+      specialize (IHc' (S m) (fun st => if e st then 1 else 0) H0 st).
+      rewrite Hc in IHc'. simpl in IHc'.
+      generalize (@wpf_infer_f c (indicator e) (S m) H0 st).
+      unfold compose, evalCompile, evalState; rewrite Hc; auto.
+      apply label_in_not_in; intro HC. apply label_in_bound_or_free in HC.
+      destruct HC as [HC|HC].
+      * eapply compile_bound_labels in Hc; eauto; lia.
+      * eapply compile_free_in_0 in Hc; eauto; lia.
+      * eapply compile_wf_tree'; eauto.
+    + specialize (IHc' (S m) g H0 st).
+      rewrite IHc'. rewrite Hc. simpl.
+      unfold g. unfold k.
+      rewrite infer_f_lib_bind_fail.
+      * reflexivity.
+      * apply bound_in_not_bound_in; intro HC.
+        eapply compile_bound_labels in Hc; eauto; lia.
+  - destruct (e st); reflexivity.
+Qed.
+
+Lemma cwpf_infer c f n :
+  wf_cpGCL c ->
+  cwpf c f ==f infer f ∘ evalCompile c n.
+Proof.
+  intros Hwf x.
+  unfold cwpf, infer, compose; simpl.
+  apply Qeq_Qdiv.
+  - apply wpf_infer_f; auto.
+  - apply wlpf_infer_f_lib; auto.
+Qed.
