theory/cwp/tests.v
@@ -1,5 +1,7 @@
-Set Implicit Arguments.
+(** Testing functional CWP and compilation+inference on example
+    programs.  *)
 
+Set Implicit Arguments.
 Require Import Coq.Program.Basics.
 Require Import Coq.QArith.QArith.
 
@@ -28,7 +30,7 @@ Definition ex1_f := fun st => if st O : bool then 1 else 0.
 Example ex1 : infer ex1_f goldfish_piranha_tree == 2#3.
 Proof. reflexivity. Qed.
 Example ex2 : infer ex1_f goldfish_piranha_tree ==
-              cwp_iid goldfish_piranha ex1_f empty.
+              cwpf goldfish_piranha ex1_f empty.
 Proof. reflexivity. Qed.
 
 Definition test_abort : cpGCL :=
@@ -41,25 +43,25 @@ Definition test_abort_tree : tree St := evalCompile' test_abort empty.
 Definition ex3_f := fun st => if st O : bool then 1 else 0.
 Example ex3 : infer ex3_f test_abort_tree == 1#3.
 Proof. reflexivity. Qed.
-Example ex4 : infer ex3_f test_abort_tree == cwp_iid test_abort ex3_f empty.
+Example ex4 : infer ex3_f test_abort_tree == cwpf test_abort ex3_f empty.
 Proof. reflexivity. Qed.
 
 Definition ex5_f := fun st => if st O : bool then 1 else 0.
 Example ex5 : infer ex5_f test_abort_tree == 1#3.
 Proof. reflexivity. Qed.
-Example ex6 : infer ex5_f test_abort_tree == cwp_iid test_abort ex5_f empty.
+Example ex6 : infer ex5_f test_abort_tree == cwpf test_abort ex5_f empty.
 Proof. reflexivity. Qed.
 
 Definition ex7_f := fun st => if negb (st O) then 1 else 0.
 Example ex7 : infer ex7_f test_abort_tree == 0.
 Proof. reflexivity. Qed.
-Example ex8 : infer ex7_f test_abort_tree == cwp_iid test_abort ex7_f empty.
+Example ex8 : infer ex7_f test_abort_tree == cwpf test_abort ex7_f empty.
 Proof. reflexivity. Qed.
 
 Example ex9 : infer (const 1) test_abort_tree == 1#3.
 Proof. reflexivity. Qed.
 Example ex10 : infer (const 1) test_abort_tree ==
-               cwp_iid test_abort (const 1) empty.
+               cwpf test_abort (const 1) empty.
 Proof. reflexivity. Qed.
 
 (** infer_f (const 1) yields the probability of terminating. *)
@@ -73,14 +75,14 @@ Definition ex13_f := fun st => if st O : bool then 1 else 0.
 Example ex13 : infer ex13_f test_abort_tree == 1#3.
 Proof. reflexivity. Qed.
 Example ex14 : infer ex13_f test_abort_tree ==
-               cwp_iid test_abort ex13_f empty.
+               cwpf test_abort ex13_f empty.
 Proof. reflexivity. Qed.
 
 Definition ex15_c := CChoice (1#2) CSkip CAbort.
 Example ex15 : infer (const 1) (evalCompile' ex15_c empty) == 1#2.
 Proof. reflexivity. Qed.
 Example ex16 : infer (const 1) (evalCompile' ex15_c empty) ==
-               cwp_iid ex15_c (const 1) empty.
+               cwpf ex15_c (const 1) empty.
 Proof. reflexivity. Qed.
 
 Definition fair_coin : cpGCL :=
@@ -94,7 +96,7 @@ Definition fair_coin_tree : tree St := evalCompile' fair_coin empty.
 Definition ex17_f := fun st => if st O : bool then 1 else 0.
 Example ex17 : infer ex17_f fair_coin_tree == 1#2.
 Proof. reflexivity. Qed.
-Example ex18 : infer ex17_f fair_coin_tree == cwp_iid fair_coin ex17_f empty.
+Example ex18 : infer ex17_f fair_coin_tree == cwpf fair_coin ex17_f empty.
 Proof. reflexivity. Qed.
 
 Definition two_thirds_loop (x : nat) (z : nat) : cpGCL :=
@@ -121,6 +123,6 @@ Definition ex19_f := fun st => if st O : bool then 1 else 0.
 Example ex19 : infer ex19_f fair_coin_loop_tree == 1#2.
 Proof. reflexivity. Qed.
 Example ex20 : infer ex19_f fair_coin_loop_tree ==
-               cwp_iid fair_coin_loop ex19_f empty.
+               cwpf fair_coin_loop ex19_f empty.
 Proof. reflexivity. Qed.
 
